Filled some holes, generalized SPEC of NISTseed wrt protocol state of HMAC component, ...

hmacdrbg/DRBG_functions.v
@@ -5,7 +5,12 @@ Require Import hmacdrbg.entropy.
 Definition DRBG_working_state: Type := (list Z * list Z * Z)%type. (* value * key * reseed_counter *)
 Definition DRBG_state_handle: Type := (DRBG_working_state * Z * bool)%type. (* state, security_strength, prediction_resistance_flag *)
 
-Definition DRBG_instantiate_function (instantiate_algorithm: list Z -> list Z -> list Z -> Z -> DRBG_working_state) (min_entropy_length max_entropy_length: Z) (provided_nonce: option (list Z)) (highest_supported_security_strength: Z) (max_personalization_string_length: Z) (prediction_resistance_supported: bool) (entropy_stream: ENTROPY.stream) (requested_instantiation_security_strength: Z) (prediction_resistance_flag: bool) (personalization_string: list Z): ENTROPY.result DRBG_state_handle :=
+Definition DRBG_instantiate_function (instantiate_algorithm: list Z -> list Z -> list Z -> Z -> DRBG_working_state)
+            (min_entropy_length max_entropy_length: Z) (provided_nonce: option (list Z))
+            (highest_supported_security_strength: Z) (max_personalization_string_length: Z)
+            (prediction_resistance_supported: bool) (entropy_stream: ENTROPY.stream) 
+            (requested_instantiation_security_strength: Z) (prediction_resistance_flag: bool) 
+            (personalization_string: list Z): ENTROPY.result DRBG_state_handle :=
   if requested_instantiation_security_strength >? highest_supported_security_strength then ENTROPY.error ENTROPY.generic_error entropy_stream
   else match prediction_resistance_flag, prediction_resistance_supported with
          | true, false => ENTROPY.error ENTROPY.generic_error entropy_stream
@@ -25,7 +30,8 @@ Definition DRBG_instantiate_function (instantiate_algorithm: list Z -> list Z ->
                  | ENTROPY.success entropy_input entropy_stream =>
                    let nonce_result := match provided_nonce with
                                          | Some n => ENTROPY.success n entropy_stream
-                                         | None => get_entropy (security_strength/2) (min_entropy_length/2) (max_entropy_length/2) prediction_resistance_flag entropy_stream
+                                         | None => get_entropy (security_strength/2) (min_entropy_length/2) (max_entropy_length/2)
+                                                               prediction_resistance_flag entropy_stream
                                        end in
                    match nonce_result with
                      | ENTROPY.error e s' => ENTROPY.error ENTROPY.catastrophic_error s'
@@ -37,13 +43,16 @@ Definition DRBG_instantiate_function (instantiate_algorithm: list Z -> list Z ->
              end
        end.
 
-Definition DRBG_reseed_function (reseed_algorithm: DRBG_working_state -> list Z -> list Z -> DRBG_working_state) (min_entropy_length max_entropy_length: Z) (max_additional_input_length: Z) (entropy_stream: ENTROPY.stream) (state_handle: DRBG_state_handle) (prediction_resistance_request: bool) (additional_input: list Z): ENTROPY.result DRBG_state_handle :=
+Definition DRBG_reseed_function (reseed_algorithm: DRBG_working_state -> list Z -> list Z -> DRBG_working_state)
+            (min_entropy_length max_entropy_length: Z) (max_additional_input_length: Z)
+            (entropy_stream: ENTROPY.stream) (state_handle: DRBG_state_handle)
+            (prediction_resistance_request: bool) (additional_input: list Z): ENTROPY.result DRBG_state_handle :=
   match state_handle with (working_state, security_strength, prediction_resistance_flag) =>
   if prediction_resistance_request && (negb prediction_resistance_flag) then ENTROPY.error ENTROPY.generic_error entropy_stream
   else
     if Zlength additional_input >? max_additional_input_length then ENTROPY.error ENTROPY.generic_error entropy_stream
     else
-      match get_entropy security_strength min_entropy_length max_entropy_length prediction_resistance_flag entropy_stream with
+      match get_entropy security_strength min_entropy_length max_entropy_length prediction_resistance_request entropy_stream with
         | ENTROPY.error _ s => ENTROPY.error ENTROPY.catastrophic_error s
         | ENTROPY.success entropy_input entropy_stream =>
           let new_working_state := reseed_algorithm working_state entropy_input additional_input in
@@ -55,7 +64,10 @@ Inductive DRBG_generate_algorithm_result :=
 | generate_algorithm_reseed_required: DRBG_generate_algorithm_result
 | generate_algorithm_success: list Z -> DRBG_working_state -> DRBG_generate_algorithm_result.
 
-Fixpoint DRBG_generate_function_helper (generate_algorithm: DRBG_working_state -> Z -> list Z -> DRBG_generate_algorithm_result) (reseed_function: ENTROPY.stream -> DRBG_state_handle -> bool -> list Z -> ENTROPY.result DRBG_state_handle) (entropy_stream: ENTROPY.stream) (state_handle: DRBG_state_handle) (requested_number_of_bytes: Z) (prediction_resistance_request: bool) (additional_input: list Z) (should_reseed: bool) (count: nat): ENTROPY.result (list Z * DRBG_working_state) :=
+Fixpoint DRBG_generate_function_helper (generate_algorithm: DRBG_working_state -> Z -> list Z -> DRBG_generate_algorithm_result)
+          (reseed_function: ENTROPY.stream -> DRBG_state_handle -> bool -> list Z -> ENTROPY.result DRBG_state_handle)
+          (entropy_stream: ENTROPY.stream) (state_handle: DRBG_state_handle) (requested_number_of_bytes: Z)
+          (prediction_resistance_request: bool) (additional_input: list Z) (should_reseed: bool) (count: nat): ENTROPY.result (list Z * DRBG_working_state) :=
   let result := if should_reseed then
                         match reseed_function entropy_stream state_handle prediction_resistance_request additional_input with
                           | ENTROPY.success x entropy_stream => ENTROPY.success (x, []) entropy_stream
@@ -70,14 +82,21 @@ Fixpoint DRBG_generate_function_helper (generate_algorithm: DRBG_working_state -
           | generate_algorithm_reseed_required =>
             match count with
               | O => ENTROPY.error ENTROPY.generic_error entropy_stream (* impossible *)
-              | S count' => DRBG_generate_function_helper generate_algorithm reseed_function entropy_stream state_handle requested_number_of_bytes prediction_resistance_request additional_input true count'
+              | S count' => DRBG_generate_function_helper generate_algorithm reseed_function 
+                                entropy_stream state_handle requested_number_of_bytes
+                                prediction_resistance_request additional_input true count'
             end
           | generate_algorithm_success x y => ENTROPY.success (x, y) entropy_stream
         end
       end
     end.
 
-Definition DRBG_generate_function (generate_algorithm: Z -> DRBG_working_state -> Z -> list Z -> DRBG_generate_algorithm_result) (reseed_function: ENTROPY.stream -> DRBG_state_handle -> bool -> list Z -> ENTROPY.result DRBG_state_handle) (reseed_interval: Z) (max_number_of_bytes_per_request: Z) (max_additional_input_length: Z) (entropy_stream: ENTROPY.stream) (state_handle: DRBG_state_handle) (requested_number_of_bytes requested_security_strength: Z) (prediction_resistance_request: bool) (additional_input: list Z): ENTROPY.result (list Z * DRBG_state_handle) :=
+Definition DRBG_generate_function (generate_algorithm: Z -> DRBG_working_state -> Z -> list Z -> DRBG_generate_algorithm_result) 
+             (reseed_function: ENTROPY.stream -> DRBG_state_handle -> bool -> list Z -> ENTROPY.result DRBG_state_handle) 
+             (reseed_interval: Z) (max_number_of_bytes_per_request: Z) (max_additional_input_length: Z)
+             (entropy_stream: ENTROPY.stream) (state_handle: DRBG_state_handle) 
+             (requested_number_of_bytes requested_security_strength: Z) 
+             (prediction_resistance_request: bool) (additional_input: list Z): ENTROPY.result (list Z * DRBG_state_handle) :=
   match state_handle with (working_state, security_strength, prediction_resistance_flag) =>
     if requested_number_of_bytes >? max_number_of_bytes_per_request then ENTROPY.error ENTROPY.generic_error entropy_stream
     else
@@ -87,7 +106,9 @@ Definition DRBG_generate_function (generate_algorithm: Z -> DRBG_working_state -
         else
           if prediction_resistance_request && (negb prediction_resistance_flag) then ENTROPY.error ENTROPY.generic_error entropy_stream
           else
-            match DRBG_generate_function_helper (generate_algorithm reseed_interval) reseed_function entropy_stream state_handle requested_number_of_bytes prediction_resistance_request additional_input prediction_resistance_request 1%nat with
+            match DRBG_generate_function_helper (generate_algorithm reseed_interval) reseed_function 
+                       entropy_stream state_handle requested_number_of_bytes prediction_resistance_request
+                       additional_input prediction_resistance_request 1%nat with
               | ENTROPY.error e s => ENTROPY.error e s
               | ENTROPY.success (output, new_working_state) entropy_stream =>
                   ENTROPY.success (output, (new_working_state, security_strength, prediction_resistance_flag)) entropy_stream
