hmacdrbg/verif_hmac_drbg_NISTseed.v
@@ -18,8 +18,6 @@ Require Import hmacdrbg.spec_hmac_drbg.
 Require Import hmacdrbg.HMAC_DRBG_common_lemmas.
 Require Import hmacdrbg.spec_hmac_drbg_pure_lemmas.
 
-Lemma FALSE: False. Admitted. (*FOR THE ONE TEMPORARY ADMIT IN THIS PROOF*)
-
 (*TEMPORARRY FIX TO DEAL WITH NAME SPACES*)
 Axiom FINALNAME:_HMAC_Final = hmac._HMAC_Final. 
 Axiom UPDATENAME:_HMAC_Update = hmac._HMAC_Update. 
@@ -39,11 +37,16 @@ Axiom Entropy_addSuccess2: forall n m s s1 l1 s2 e,
 Axiom Entropy_addError: forall n m s s1 e, ENTROPY.get_bytes n s = ENTROPY.error e s1 ->
         ENTROPY.get_bytes (n+m) s = ENTROPY.error e s1.
 
-(*Entropy_add is derivable from Entropy_addStrong:*)
-Goal forall n m s s1 s2 x1 x2, ENTROPY.get_bytes n s = ENTROPY.success x1 s1 ->
-        ENTROPY.get_bytes m s1 = ENTROPY.success x2 s2 ->
-        exists x, ENTROPY.get_bytes (n+m) s = ENTROPY.success x s2.
-Proof. intros. rewrite (Entropy_addSuccess1 _ _ _ _ _ _ _ H H0). eexists; trivial. Qed.
+Lemma Entropy_le n s l ss: ENTROPY.success l ss = ENTROPY.get_bytes n s ->
+  forall m, (m <= n)%nat -> exists l' s', ENTROPY.success l' s' = ENTROPY.get_bytes m s.
+Proof. intros.
+  remember (ENTROPY.get_bytes m s) as d.
+  destruct d. eexists; eexists; trivial.
+  symmetry in H; symmetry in Heqd.
+  specialize (Entropy_addError _ (n-m)%nat _ _ _ Heqd).
+     rewrite le_plus_minus_r; trivial.
+  intros HH; rewrite HH in *. discriminate.
+Qed.
 
 Definition OptionalNonce: option (list Z) := None. (*The implementation takes nonce from entropy, using the el*3/2 calculation*)
 
@@ -51,66 +54,200 @@ Parameter max_personalization_string_length: Z. (*NIST SP 800-90A, page 38, Tabl
          Our personalization string is a list of bytes, so have max length 2^32*)
 Axiom max_personalization_string336: 336 <= max_personalization_string_length.
 
-Parameter prediction_resistance_supported: bool.
+Definition prediction_resistance_supported:bool:=true.
 
 (*NIST, Section 10.1: highest supported sec strength is given by the has function's
 security strength for preimage resistance. For SHA256, this is 
 (according to NIST SP 800-107, Table 1, page 11) 256 bits*)
-Definition highest_supported_security_strength := 256. (*as in reseed; so in bits - but should it be in bytes?*)
-
+Definition highest_supported_security_strength := 32. (* in bytes -- see comment for reseed*)
 
 (*Q: should we use the sec strength of HMAC, calculated according to Section 5.3.4 of 
 NIST SP 800-107 instead?*)
-Definition requested_instantiation_security_strength:= 32.  (*is this right?*)
+Definition requested_security_strength:= 32.  (*same as in reseed*)
 
-Definition mbedtls_HMAC256_DRBG_init_function (entropy_stream: ENTROPY.stream) 
-         entropy_len prediction_resistance (personalization_string: list Z): ENTROPY.result DRBG_state_handle :=
+Definition mbedtls_HMAC256_DRBG_instantiate_function (entropy_stream: ENTROPY.stream) 
+         entropy_len pr_flag (personalization_string: list Z): ENTROPY.result DRBG_state_handle :=
    let reseed_interval := 10000 
    in HMAC256_DRBG_instantiate_function entropy_len entropy_len OptionalNonce
             highest_supported_security_strength max_personalization_string_length
             prediction_resistance_supported entropy_stream
-            requested_instantiation_security_strength prediction_resistance personalization_string.
+            requested_security_strength pr_flag personalization_string.
 
 Definition entlen:Z := 32.
 
+Definition MD_ANY (r: mdstate): mpred :=
+  (md_empty r) || (EX h:_, md_relate h r) || (EX k:_, md_full k r). 
 (*
-Inductive md_any (r: mdstate): mpred :=
-  md_any_empty: md_empty r -> md_any r.
-| md_any_rep: forall h r, md_relate h r -> md_any r
-| md_any_full: forall k r, md_full k r -> md_any r.
+Require Import msl.predicates_hered.
+
+Inductive md_any (r: mdstate): compcert_rmaps.RML.R.rmap -> Prop:= 
+  md_any_empty: forall phi, app_pred (md_empty r) phi -> md_any r phi
+| md_any_rep: forall h phi, app_pred (md_relate h r) phi -> md_any r phi
+| md_any_full: forall k phi, app_pred (md_full k r) phi -> md_any r phi.
+
+Definition MDANY (r:mdstate):mpred.
+refine (exist _ (md_any r) _). red; intros.
+inv H0.
+apply md_any_empty. destruct (md_empty r); simpl in *. eapply h; eauto.
+apply (md_any_rep r h). destruct (md_relate h r); simpl in *. eapply h0; eauto.
+apply (md_any_full r k). destruct (md_full k r); simpl in *. eapply h; eauto.
+Defined.
+
+Lemma inject_md_any_empty r: md_empty r |-- MDANY r. 
+constructor; trivial. Qed.
+Lemma inject_md_any_rep h r: md_relate h r |-- MDANY r. 
+red; intros. eapply md_any_rep; eassumption. Qed. 
+Lemma inject_md_any_full k r: md_full k r |-- MDANY r. 
+red; intros. eapply md_any_full; eassumption. Qed.
+
+Lemma MDANY_elim r: MDANY r |-- MD_ANY r.
+unfold MD_ANY.
+red; intros. inv H.
++ eapply orp_right1. 2: apply H0.
+  eapply orp_right1. apply derives_refl. 
++ eapply orp_right1. 2: apply H0. 
+  eapply orp_right2. econstructor. apply H.
++ eapply orp_right2. 2: apply H0. 
+  econstructor. apply H.
+Qed. 
+
+Lemma MDANY_intros r: MD_ANY r |-- MDANY r.
+unfold MD_ANY.
+rewrite orp_is_exp. apply exp_left; intros.
+destruct x.
++ rewrite orp_is_exp. apply exp_left; intros.
+  destruct x.
+  - apply inject_md_any_empty.
+  - apply exp_left; intros. eapply inject_md_any_rep.
++ apply exp_left; intros. eapply inject_md_any_full.
+Qed.
 *)
 
-Definition preseed_relate rc pr ri (r : hmac256drbgstate):mpred:=
+Lemma ReseedRes: forall X r v, @return_value_relate_result X r (Vint v) -> Int.eq v (Int.repr (-20864)) = false.
+Proof. intros.
+  unfold return_value_relate_result in H.
+  destruct r. inv H; reflexivity.
+  destruct e; inv H; try reflexivity.
+  apply Int.eq_false. eapply ENT_GenErrAx. 
+Qed.
+
+Lemma instantiate_reseed d s pr_flag rc ri (ZLc'256F : (Zlength d >? 256) = false):
+      mbedtls_HMAC256_DRBG_instantiate_function s entlen pr_flag  d =
+      mbedtls_HMAC256_DRBG_reseed_function s (HMAC256DRBGabs initial_key initial_value rc 48 pr_flag ri) d.
+Proof. intros. 
+  unfold mbedtls_HMAC256_DRBG_instantiate_function, HMAC256_DRBG_instantiate_function,
+       DRBG_instantiate_function, mbedtls_HMAC256_DRBG_reseed_function; simpl. 
+  rewrite ZLc'256F, andb_negb_r.
+  assert (MaxString': Zlength d >? max_personalization_string_length = false).
+  { apply Zgt_is_gt_bool_f. apply Zgt_is_gt_bool_f in ZLc'256F.
+    specialize max_personalization_string336; intros; omega. }
+  rewrite MaxString' in *; clear.
+  destruct pr_flag; simpl in *. 
+  + unfold get_entropy, entlen. 
+    remember (ENTROPY.get_bytes (Z.to_nat 48) s) as ENT.
+    destruct ENT.
+    - destruct (Entropy_le _ _ _ _ HeqENT (Z.to_nat 32)) as [l32 [s32 Ent32]]; try (simpl; omega).
+      symmetry in Ent32; rewrite Ent32. 
+      change (32 / 2) with 16 in *.
+      remember (ENTROPY.get_bytes (Z.to_nat 16) s32) as  ENT2; symmetry in HeqENT2.
+      destruct ENT2.
+      * specialize (Entropy_addSuccess1 _ 16 _ _ _ _ _ Ent32 HeqENT2); intros XX.
+        simpl in *; rewrite XX in *; clear XX. inv HeqENT.
+        f_equal. unfold HMAC256_DRBG_instantiate_algorithm, HMAC_DRBG_instantiate_algorithm.
+        rewrite app_assoc; trivial.
+      * specialize (Entropy_addSuccess2 _ 16 _ _ _ _ _ Ent32 HeqENT2); intros XX.
+        simpl in *; rewrite XX in *; clear XX. inv HeqENT.
+    - remember (ENTROPY.get_bytes (Z.to_nat 32) s) as Ent32; symmetry in HeqEnt32.
+      destruct Ent32.
+      * change (32 / 2) with 16 in *.
+        remember (ENTROPY.get_bytes (Z.to_nat 16) s1) as  ENT2; symmetry in HeqENT2.
+        destruct ENT2.
+        ++ specialize (Entropy_addSuccess1 _ 16 _ _ _ _ _ HeqEnt32 HeqENT2); intros XX.
+           simpl in *; rewrite XX in *; clear XX. inv HeqENT.
+        ++ specialize (Entropy_addSuccess2 _ 16 _ _ _ _ _ HeqEnt32 HeqENT2); intros XX.
+           simpl in *; rewrite XX in *; clear XX. inv HeqENT. trivial.
+      * specialize (Entropy_addError _ 16 _ _ _ HeqEnt32); intros XX.
+        simpl in *; rewrite XX in *; clear XX. inv HeqENT. trivial.
+  + (*same proof...*)
+    unfold get_entropy, entlen. 
+    remember (ENTROPY.get_bytes (Z.to_nat 48) s) as ENT.
+    destruct ENT.
+    - destruct (Entropy_le _ _ _ _ HeqENT (Z.to_nat 32)) as [l32 [s32 Ent32]]; try (simpl; omega).
+      symmetry in Ent32; rewrite Ent32. 
+      change (32 / 2) with 16 in *.
+      remember (ENTROPY.get_bytes (Z.to_nat 16) s32) as  ENT2; symmetry in HeqENT2.
+      destruct ENT2.
+      * specialize (Entropy_addSuccess1 _ 16 _ _ _ _ _ Ent32 HeqENT2); intros XX.
+        simpl in *; rewrite XX in *; clear XX. inv HeqENT.
+        f_equal. unfold HMAC256_DRBG_instantiate_algorithm, HMAC_DRBG_instantiate_algorithm.
+        rewrite app_assoc; trivial.
+      * specialize (Entropy_addSuccess2 _ 16 _ _ _ _ _ Ent32 HeqENT2); intros XX.
+        simpl in *; rewrite XX in *; clear XX. inv HeqENT.
+    - remember (ENTROPY.get_bytes (Z.to_nat 32) s) as Ent32; symmetry in HeqEnt32.
+      destruct Ent32.
+      * change (32 / 2) with 16 in *.
+        remember (ENTROPY.get_bytes (Z.to_nat 16) s1) as  ENT2; symmetry in HeqENT2.
+        destruct ENT2.
+        ++ specialize (Entropy_addSuccess1 _ 16 _ _ _ _ _ HeqEnt32 HeqENT2); intros XX.
+           simpl in *; rewrite XX in *; clear XX. inv HeqENT.
+        ++ specialize (Entropy_addSuccess2 _ 16 _ _ _ _ _ HeqEnt32 HeqENT2); intros XX.
+           simpl in *; rewrite XX in *; clear XX. inv HeqENT. trivial.
+      * specialize (Entropy_addError _ 16 _ _ _ HeqEnt32); intros XX.
+        simpl in *; rewrite XX in *; clear XX. inv HeqENT. trivial.
+Qed. 
+
+Opaque mbedtls_HMAC256_DRBG_reseed_function.
+Opaque initial_key. Opaque initial_value.
+
+Inductive deep_any:= 
+  deep_any_empty: deep_any
+| deep_any_rep: forall h:HABS, deep_any
+| deep_any_full: forall k:list Z, deep_any.
+
+Definition deep_interp (d:deep_any) (r: mdstate):mpred :=
+  match d with
+    deep_any_empty => md_empty r 
+  | deep_any_rep h => md_relate h r
+  | deep_any_full k => md_full k r
+  end.
+   
+Lemma deep_interp_empty d r: deep_interp d r |-- md_empty r.
+destruct d; simpl. trivial.
++ destruct h. simpl. 
+  eapply derives_trans. 
+  apply protocol_spec_hmac.OPENSSL_HMAC_ABSTRACT_SPEC.REP_FULL. 
+  apply protocol_spec_hmac.OPENSSL_HMAC_ABSTRACT_SPEC.FULL_EMPTY.
++ apply protocol_spec_hmac.OPENSSL_HMAC_ABSTRACT_SPEC.FULL_EMPTY.
+Qed.  
+
+Definition preseed_relate d rc pr ri (r : hmac256drbgstate):mpred:=
     match r with
      (md_ctx', (V', (reseed_counter', (entropy_len', (prediction_resistance', reseed_interval'))))) =>
-    md_empty md_ctx' &&
+    deep_interp d md_ctx' &&
     !! (map Vint (map Int.repr initial_key) = V' /\
-        Vint (Int.repr rc) = reseed_counter'(* /\
-        Vint (Int.repr entropy_len) = entropy_len'*) /\
+        (Vint (Int.repr rc) = reseed_counter')  (*Explicitly reset in sucessful runs of reseed and hence seed*)
+        (*Vint (Int.repr entropy_len) = entropy_len' Explicitly set in seed*) /\
         Vint (Int.repr ri) = reseed_interval' /\
         Val.of_bool pr = prediction_resistance')
    end.
  
 Definition hmac_drbg_seed_spec :=
   DECLARE _mbedtls_hmac_drbg_seed
-   WITH ctx: val, info:val, len: Z, data:val, Data: list Z,
+   WITH dp:_, ctx: val, info:val, len: Z, data:val, Data: list Z,
         Ctx: hmac256drbgstate,
-        (*CTX: hmac256drbgabs,*)
-        kv: val, Info: md_info_state, s:ENTROPY.stream, rc:Z, pr:bool, ri:Z
+        kv: val, Info: md_info_state, s:ENTROPY.stream, rc:Z, pr_flag:bool, ri:Z
     PRE [_ctx OF tptr (Tstruct _mbedtls_hmac_drbg_context noattr),
          _md_info OF tptr (Tstruct _mbedtls_md_info_t noattr),
          _custom OF tptr tuchar, _len OF tuint ] 
-       PROP ( pr = prediction_resistance_supported (*For now*) /\
-              (len = Zlength Data) /\ 
-              0 <= len (*<= 336 Int.max_unsigned*) /\
+       PROP ( (len = Zlength Data) /\ 
+              0 <= len /\
               48 + len < Int.modulus /\
               0 < 48 + Zlength (contents_with_add data len Data) < Int.modulus /\ Forall isbyteZ Data)
        LOCAL (temp _ctx ctx; temp _md_info info; 
               temp _len (Vint (Int.repr len)); temp _custom data; gvar sha._K256 kv)
        SEP (
          data_at Tsh t_struct_hmac256drbg_context_st Ctx ctx;
-         preseed_relate rc pr ri Ctx;
-         (*hmac256drbg_relate CTX Ctx;*)
+         preseed_relate dp rc pr_flag ri Ctx;
          data_at Tsh t_struct_mbedtls_md_info Info info;
          da_emp Tsh (tarray tuchar (Zlength Data)) (map Vint (map Int.repr Data)) data;
          K_vector kv; Stream s)
@@ -123,8 +260,7 @@ Definition hmac_drbg_seed_spec :=
             K_vector kv;
             if Int.eq ret_value (Int.repr (-20864))
             then data_at Tsh t_struct_hmac256drbg_context_st Ctx ctx *
-                  (*hmac256drbg_relate CTX Ctx *) preseed_relate rc pr ri Ctx * 
-                  Stream s
+                 preseed_relate dp rc pr_flag ri Ctx * Stream s
             else md_empty (fst Ctx) * 
                  EX p:val, 
                  match (fst Ctx) with (M1, (M2, M3)) =>
@@ -132,14 +268,13 @@ Definition hmac_drbg_seed_spec :=
                    then !!(ret_value = Int.repr (-5)) && 
                      (Stream s * 
                      ( let CtxFinal:= ((info, (M2, p)), (list_repeat 32 (Vint Int.one), (Vint (Int.repr rc), 
-                                       (Vint (Int.repr 48), (Val.of_bool pr, Vint (Int.repr 10000)))))) in
-                       let CTXFinal:= HMAC256DRBGabs initial_key initial_value rc 48 pr 10000 in
+                                       (Vint (Int.repr 48), (Val.of_bool pr_flag, Vint (Int.repr 10000)))))) in
+                       let CTXFinal:= HMAC256DRBGabs initial_key initial_value rc 48 pr_flag 10000 in
                        data_at Tsh t_struct_hmac256drbg_context_st CtxFinal ctx *
                                      hmac256drbg_relate CTXFinal CtxFinal))
 
-                   else (*let myABS := HMAC256DRBGabs VV initial_value rc 48 pr 10000
-                        in *) 
-                        match mbedtls_HMAC256_DRBG_init_function s entlen pr (contents_with_add data (Zlength Data) Data)
+                   else match mbedtls_HMAC256_DRBG_instantiate_function s entlen pr_flag
+                                       (contents_with_add data (Zlength Data) Data)
                         with
                          | ENTROPY.error e ss => 
                             (!!(match e with
@@ -147,8 +282,8 @@ Definition hmac_drbg_seed_spec :=
                                | ENTROPY.catastrophic_error => Vint ret_value = Vint (Int.repr (-9))
                               end) && (Stream ss * 
                                        let CtxFinal:= ((info, (M2, p)), (list_repeat 32 (Vint Int.one), (Vint (Int.repr rc), 
-                                                (Vint (Int.repr 48), (Val.of_bool pr, Vint (Int.repr 10000)))))) in
-                                       let CTXFinal:= HMAC256DRBGabs initial_key initial_value rc 48 pr 10000 in
+                                                (Vint (Int.repr 48), (Val.of_bool pr_flag, Vint (Int.repr 10000)))))) in
+                                       let CTXFinal:= HMAC256DRBGabs initial_key initial_value rc 48 pr_flag 10000 in
                                        data_at Tsh t_struct_hmac256drbg_context_st CtxFinal ctx *
                                        hmac256drbg_relate CTXFinal CtxFinal))
                         | ENTROPY.success handle ss => !!(ret_value = Int.zero) && 
@@ -161,26 +296,12 @@ Definition hmac_drbg_seed_spec :=
                         end
                 end).
 
-Lemma ReseedRes: forall X r v, @return_value_relate_result X r (Vint v) -> Int.eq v (Int.repr (-20864)) = false.
-Proof. intros.
-  unfold return_value_relate_result in H.
-  destruct r. inv H; reflexivity.
-  destruct e; inv H; try reflexivity.
-  apply Int.eq_false. eapply ENT_GenErrAx. 
-Qed.
-
-Lemma isbyteZ_initialKey: Forall isbyteZ initial_key. 
-Proof. apply Forall_list_repeat; split; omega. Qed.
-
-Opaque mbedtls_HMAC256_DRBG_reseed_function.
-Opaque initial_key. Opaque initial_value.
-
 Lemma body_hmac_drbg_seed: semax_body HmacDrbgVarSpecs HmacDrbgFunSpecs 
       f_mbedtls_hmac_drbg_seed hmac_drbg_seed_spec. 
 Proof. 
   start_function. 
   abbreviate_semax.
-  destruct H as [PREQ [HDlen1 [HDlen2 [DHlen3 [DHlen4 HData]]]]]. 
+  destruct H as (*[PREQ*) [HDlen1 [HDlen2 [DHlen3 [DHlen4 HData]]]](*]*). 
   rewrite data_at_isptr with (p:=ctx). Intros.
   destruct ctx; try contradiction.
   unfold_data_at 1%nat.
@@ -200,8 +321,9 @@ Proof.
    LOCAL (temp _ret (Vint (Int.repr v)); temp 235%positive (Vint (Int.repr v));
    temp _ctx (Vptr b i); temp _md_info info; temp _len (Vint (Int.repr len));
    temp _custom data; gvar sha._K256 kv)
-   SEP ( (EX p : val, !!field_compatible spec_hmac.t_struct_hmac_ctx_st [] p && memory_block Tsh (sizeof (Tstruct _hmac_ctx_st noattr)) p *
-          data_at Tsh (Tstruct _mbedtls_md_context_t noattr) ((*M1*)info,(M2,p)) (Vptr b i));
+   SEP ( (EX p : val, !!(*field_compatible spec_hmac.t_struct_hmac_ctx_st [] p*)
+                        malloc_compatible (sizeof (Tstruct _hmac_ctx_st noattr))p && memory_block Tsh (sizeof (Tstruct _hmac_ctx_st noattr)) p *
+          data_at Tsh (Tstruct _mbedtls_md_context_t noattr) (info,(M2,p)) (Vptr b i));
          FRZL FR0)).
   { destruct Hv; try omega. rewrite if_false; trivial. clear H. subst v.
     forward. simpl. Exists (Int.repr (-20864)). 
@@ -211,7 +333,7 @@ Proof.
     rewrite field_at_data_at. simpl.
     unfold field_address. rewrite if_true; simpl; trivial. rewrite int_add_repr_0_r; trivial. }
   { subst v. clear Hv. simpl. forward. entailer!. }
-  Intros. subst v. clear Hv. Intros p. rename H into FC_P.
+  Intros. subst v. clear Hv. Intros p. rename H into MCp. simpl in MCp.
 
   (*Alloction / md_setup succeeded. Now get md_size*)
   drop_LOCAL 0%nat.
@@ -220,7 +342,6 @@ Proof.
  
   (*call mbedtls_md_hmac_starts( &ctx->md_ctx, ctx->V, md_size )*)
   thaw FR0. subst.
-  (*rename H1 into ZL_VV. rename H2 into isbyteZ_VV.*)
   assert (ZL_VV: Zlength initial_key =32) by reflexivity.
   thaw FIELDS. 
   freeze [3;4;5;6] FIELDS1.
@@ -229,15 +350,16 @@ Proof.
   rewrite <- ZL_VV.
   freeze [0;4;5;6;8] FR2.
   replace_SEP 1 (UNDER_SPEC.EMPTY p).
-  { entailer. apply protocol_spec_hmac.OPENSSL_HMAC_ABSTRACT_SPEC.mkEmpty. 
-    clear - FC_P. unfold field_compatible in *.
-    simpl in *. exfalso. apply FALSE. (*has contradiction in hypothesis - maybe malloc does not guarantee filed_compatible_at?? Or is it a compspecs issue*) }
+  { entailer. apply protocol_spec_hmac.OPENSSL_HMAC_ABSTRACT_SPEC.mkEmpty.
+    clear - Pp MCp. destruct p; try contradiction. destruct MCp.
+    repeat split; simpl in *; trivial.
+    + omega.
+    + unfold natural_alignment in H. unfold align_attr. simpl. 
+      destruct H. exists (x * 2)%Z. omega. 
+  }
   forward_call (Vptr b i, ((info,(M2,p)):mdstate), 32, initial_key, kv, b, Int.add i (Int.repr 12)).
-(*  { rewrite ZL_VV, int_add_repr_0_r; simpl.
-    apply prop_right; repeat split; trivial.
-  }*)
   { simpl. cancel. }
-  { split; trivial. red. simpl. rewrite int_max_signed_eq (*, ZL_VV*). 
+  { split; trivial. red. simpl. rewrite int_max_signed_eq. 
     split. trivial. split. omega. rewrite two_power_pos_equiv.
     replace (2^64) with 18446744073709551616. omega. reflexivity.
     apply isbyteZ_initialKey.
@@ -247,13 +369,9 @@ Proof.
   (*call  memset( ctx->V, 0x01, md_size )*)
   freeze [0;1;3;4] FR3.
   forward_call (Tsh, Vptr b (Int.add i (Int.repr 12)), 32, Int.one).
-(*  { rewrite ZL_VV; entailer!. 
-  } *)
   { rewrite sepcon_comm. apply sepcon_derives. 
-      eapply derives_trans. apply data_at_memory_block. 
-        rewrite ZL_VV. simpl. cancel. cancel. }
-  (*{ split. apply semax_call.writable_share_top.
-    rewrite ZL_V0, client_lemmas.int_max_unsigned_eq. omega. }*)
+     - apply data_at_memory_block. 
+     - cancel. }
 
   (*ctx->reseed_interval = MBEDTLS_HMAC_DRBG_RESEED_INTERVAL;*)
   rewrite ZL_VV. 
@@ -261,8 +379,6 @@ Proof.
   thaw FIELDS1. forward.
   freeze [0;4;5;6;7] FIELDS2.
   freeze [0;1;2;3;4;5;6;7;8] ALLSEP.
-
-(*  set (ent_len := new_ent_len (Zlength V0)) in *.*)
 
   forward_if 
   (PROP ( )
@@ -284,10 +400,11 @@ Proof.
       unfold overridePost.
       destruct (eq_dec ek EK_normal).
       { subst ek. (*entailer. STILL FAILS*) unfold POSTCONDITION, abbreviate.
-        normalize. (*simpl. intros.*) apply andp_left2. normalize.
-        old_go_lower.
-        normalize. Time entailer. }
-      { apply andp_left2. cancel. }
+        normalize. (*simpl. intros.*) (*apply andp_left2. normalize.*)
+        entailer!. }
+      { apply andp_left2; trivial. 
+       (*FLOYD: again, entailer fails*)
+      }
     }
   }
   forward. simpl. drop_LOCAL 7%nat. (*237%positive*) 
@@ -298,11 +415,10 @@ Proof.
   assert (FOURTYEIGHT: Int.unsigned (Int.mul (Int.repr 32) (Int.repr 3)) / 2 = 48).
   { rewrite mul_repr. simpl.
     rewrite Int.unsigned_repr. reflexivity. rewrite int_max_unsigned_eq; omega. }
-  set (pr:= prediction_resistance_supported) in *.
-  set (myABS := HMAC256DRBGabs initial_key initial_value rc 48 pr  10000) in *. 
+  set (myABS := HMAC256DRBGabs initial_key initial_value rc 48 pr_flag 10000) in *. 
   assert (myST: exists ST:hmac256drbgstate, ST = 
     ((info, (M2, p)), (map Vint (list_repeat 32 Int.one), (Vint (Int.repr rc),
-        (Vint (Int.repr 48), (Val.of_bool pr, Vint (Int.repr 10000))))))). eexists; reflexivity.
+        (Vint (Int.repr 48), (Val.of_bool pr_flag, Vint (Int.repr 10000))))))). eexists; reflexivity.
   destruct myST as [ST HST].
 
   freeze [0;1;2;3;4] FR_CTX.
@@ -320,9 +436,10 @@ Proof.
     apply andp_right. apply prop_right. repeat split; trivial. apply IB1. split; omega. 
     unfold md_full. simpl.
     rewrite field_at_data_at. simpl.
-    unfold field_address. rewrite if_true; simpl; trivial. rewrite int_add_repr_0_r. cancel.
+    unfold field_address. rewrite if_true; simpl; trivial.
     rewrite field_at_data_at. simpl.
-    unfold field_address. rewrite if_true; simpl; trivial. cancel. 
+    unfold field_address. rewrite if_true; simpl; trivial. 
+    rewrite int_add_repr_0_r; cancel.
     apply protocol_spec_hmac.OPENSSL_HMAC_ABSTRACT_SPEC.REP_FULL.
   }
 
@@ -349,6 +466,7 @@ Proof.
                  Zlength (contents_with_add data (Zlength Data) Data) = Zlength Data).
          { unfold contents_with_add. if_tac. right; trivial. left; trivial. }
   forward. 
+
   forward_if (
    PROP ( v = nullval)
    LOCAL (temp _ret v; temp 240%positive v;
@@ -371,6 +489,7 @@ Proof.
       simpl. subst myABS. normalize. simpl. cancel.
       Exists p. thaw OLD_MD. normalize. 
       apply andp_right. apply prop_right; repeat split; trivial. cancel.
+      apply deep_interp_empty.
     + destruct (zlt 384 (48 + Zlength Data)); simpl in Heqd; try omega. 
       subst d.
       unfold hmac256drbgstate_md_info_pointer, hmac256drbg_relate; simpl. normalize.
@@ -385,45 +504,12 @@ Proof.
       destruct MRS.
       - exfalso. inv RV. simpl in Hv. discriminate.
       - simpl. normalize. Exists p. thaw OLD_MD. cancel.
-        remember (mbedtls_HMAC256_DRBG_init_function s entlen pr (contents_with_add data (Zlength Data) Data)) as INIT.
-        assert (ERR: INIT = ENTROPY.error ENTROPY.catastrophic_error s0 /\
-                  e = ENTROPY.catastrophic_error).
-        { unfold mbedtls_HMAC256_DRBG_init_function, HMAC256_DRBG_instantiate_function, DRBG_instantiate_function in HeqINIT; simpl in HeqINIT.
-Transparent mbedtls_HMAC256_DRBG_reseed_function.
-          unfold mbedtls_HMAC256_DRBG_reseed_function in HeqMRS. 
-Opaque mbedtls_HMAC256_DRBG_reseed_function.
-          subst myABS. simpl in HeqMRS. rewrite ZLc'256F in *. subst pr. rewrite andb_negb_r in *.
-          assert (MaxString': Zlength (contents_with_add data (Zlength Data) Data) >?
-                    max_personalization_string_length = false).
-          { apply Zgt_is_gt_bool_f. specialize max_personalization_string336; intros.
-            destruct ZLc' as [ZLc' | ZLc']; rewrite ZLc'; trivial; omega. }
-          rewrite MaxString' in *.
-          destruct prediction_resistance_supported; simpl in *.
-          ++ unfold get_entropy in *. clear - g0 HeqMRS HeqINIT. unfold entlen in *. 
-             remember (ENTROPY.get_bytes (Z.to_nat 48) s) as ENT. destruct ENT; try discriminate. 
-             inv HeqMRS.
-             remember (ENTROPY.get_bytes (Z.to_nat 32) s) as  ENT1; symmetry in HeqENT1.
-             destruct ENT1; try discriminate. change (32 / 2) with 16 in *.
-             remember (ENTROPY.get_bytes (Z.to_nat 16) s0) as  ENT2; symmetry in HeqENT2.
-             destruct ENT2; try discriminate.
-             specialize (Entropy_addSuccess1 _ 16 _ _ _ _ _ HeqENT1 HeqENT2); intros XX. simpl in *; rewrite XX in *; clear XX; discriminate.
-             specialize (Entropy_addSuccess2 _ 16 _ _ _ _ _ HeqENT1 HeqENT2); intros XX. simpl in *; rewrite XX in *; clear XX. inv HeqENT. split; trivial.
-             specialize (Entropy_addError _ 16 _ _ _ HeqENT1); intros XX. simpl in *; rewrite XX in *; clear XX. inv HeqENT. split; trivial.
-          ++ unfold get_entropy in *. clear - g0 HeqMRS HeqINIT. unfold entlen in *. 
-             remember (ENTROPY.get_bytes (Z.to_nat 48) s) as ENT. destruct ENT; try discriminate. 
-             inv HeqMRS.
-             remember (ENTROPY.get_bytes (Z.to_nat 32) s) as  ENT1; symmetry in HeqENT1.
-             destruct ENT1; try discriminate. change (32 / 2) with 16 in *.
-             remember (ENTROPY.get_bytes (Z.to_nat 16) s0) as  ENT2; symmetry in HeqENT2.
-             destruct ENT2; try discriminate.
-             specialize (Entropy_addSuccess1 _ 16 _ _ _ _ _ HeqENT1 HeqENT2); intros XX. simpl in *; rewrite XX in *; clear XX; discriminate.
-             specialize (Entropy_addSuccess2 _ 16 _ _ _ _ _ HeqENT1 HeqENT2); intros XX. simpl in *; rewrite XX in *; clear XX. inv HeqENT. split; trivial.
-             specialize (Entropy_addError _ 16 _ _ _ HeqENT1); intros XX. simpl in *; rewrite XX in *; clear XX. inv HeqENT. split; trivial.
-          }
-          destruct ERR as [SS EE]. rewrite SS in *. clear SS. subst e.
-          normalize.
-          apply andp_right. apply prop_right; repeat split; trivial.
-          cancel.
+        subst myABS. rewrite <- instantiate_reseed in HeqMRS; trivial.
+        rewrite <- HeqMRS.
+        normalize.
+        apply andp_right. apply prop_right; repeat split; trivial.
+        cancel.
+        apply deep_interp_empty. 
   }
   { rename H into Hv. forward.
     go_lower. simpl in Hv. apply typed_false_of_bool in Hv. apply negb_false_iff in Hv.
@@ -437,10 +523,11 @@ Opaque mbedtls_HMAC256_DRBG_reseed_function.
   destruct d; Intros.
   remember (mbedtls_HMAC256_DRBG_reseed_function s myABS
          (contents_with_add data (Zlength Data) Data)) as MRS. 
+  unfold hmac256drbgabs_reseed. rewrite <- HeqMRS. subst myABS; simpl. 
   unfold return_value_relate_result in H.
   destruct MRS. Focus 2. exfalso. destruct e. inv H. 
                      destruct ENT_GenErrAx as [EL1 _]. rewrite <- H in EL1. elim EL1; trivial. 
-  clear H. unfold hmac256drbgabs_reseed. rewrite <- HeqMRS. subst myABS; simpl.
+  clear H.
   destruct d as [[[[newV newK] newRC] dd] newPR].
   unfold hmac256drbgabs_common_mpreds. simpl. subst ST. unfold hmac256drbgstate_md_info_pointer. simpl. Intros. 
   unfold_data_at 1%nat. freeze [0;1;2;4;5;6;7;8;9;10;11] XX.
@@ -455,55 +542,11 @@ Opaque mbedtls_HMAC256_DRBG_reseed_function.
   assert (ZLc'256F: Zlength (contents_with_add data (Zlength Data) Data) >? 256 = false).
       { destruct ZLc' as [HH | HH]; rewrite HH. reflexivity.
         apply Zgt_is_gt_bool_f. omega. } 
-  assert (MaxString': Zlength (contents_with_add data (Zlength Data) Data) >?
-                    max_personalization_string_length = false).
-          { apply Zgt_is_gt_bool_f. specialize max_personalization_string336; intros.
-            destruct ZLc' as [ZLc' | ZLc']; rewrite ZLc'; trivial; omega. }
-  remember (mbedtls_HMAC256_DRBG_init_function s entlen pr (contents_with_add data (Zlength Data) Data)) as INIT.
-  assert (INIT = ENTROPY.success (newV, newK, newRC, entlen, newPR) s0).
-  { unfold mbedtls_HMAC256_DRBG_init_function, HMAC256_DRBG_instantiate_function, DRBG_instantiate_function in HeqINIT; simpl in HeqINIT.
-Transparent mbedtls_HMAC256_DRBG_reseed_function.
-        unfold mbedtls_HMAC256_DRBG_reseed_function in HeqMRS. 
-Opaque mbedtls_HMAC256_DRBG_reseed_function.
-          rewrite MaxString' in *.
-          destruct prediction_resistance_supported; simpl in *.
-          ++ rewrite ZLc'256F in *. unfold get_entropy, entlen in *.
-             remember (ENTROPY.get_bytes (Z.to_nat 48) s) as ENT.
-             destruct ENT; inv HeqMRS.
-             remember (ENTROPY.get_bytes (Z.to_nat 32) s) as ENT1. destruct ENT1.
-             -- change (32/2) with 16. symmetry in HeqENT1.
-                remember (ENTROPY.get_bytes (Z.to_nat 16) s0) as ENT2. destruct ENT2.
-                ** symmetry in HeqENT2.
-                   specialize (Entropy_addSuccess1 _ 16 _ _ _ _ _ HeqENT1 HeqENT2); intros XX; simpl in *. 
-                   rewrite XX in HeqENT; clear XX; inv HeqENT.
-                   unfold HMAC256_DRBG_instantiate_algorithm, HMAC_DRBG_instantiate_algorithm.
-                   rewrite <- app_assoc in H4. 
-                   remember (HMAC_DRBG_update HMAC256 (l0 ++ l1 ++ contents_with_add data (Zlength Data) Data)
-                                initial_key initial_value) as q. 
-                   destruct q; inv H4; trivial.
-                ** symmetry in HeqENT2.
-                   specialize (Entropy_addSuccess2 _ 16 _ _ _ _ _ HeqENT1 HeqENT2); intros XX; simpl in *. 
-                   rewrite XX in HeqENT; clear XX; inv HeqENT.
-             -- symmetry in HeqENT1.
-                specialize (Entropy_addError _ 16 _ _ _ HeqENT1); intros XX; simpl in *.
-                rewrite XX in *; clear XX; discriminate.
-          ++ rewrite ZLc'256F in *. unfold entlen, get_entropy in *.
-             remember (ENTROPY.get_bytes (Z.to_nat 32) s) as ENT32; symmetry in HeqENT32.
-             destruct ENT32.
-             -- change (32/2) with 16 in *.
-                remember (ENTROPY.get_bytes (Z.to_nat 16) s1). destruct r; symmetry in Heqr.
-                ** specialize (Entropy_addSuccess1 _ 16 _ _ _ _ _ HeqENT32 Heqr); intros XX; simpl in *. 
-                   rewrite XX in HeqMRS; clear XX; inv HeqMRS.
-                   unfold HMAC256_DRBG_instantiate_algorithm, HMAC_DRBG_instantiate_algorithm.
-                   rewrite <- app_assoc in H4. 
-                   remember (HMAC_DRBG_update HMAC256 (l ++ l0 ++ contents_with_add data (Zlength Data) Data) initial_key initial_value) as q.
-                    destruct q; inv H4; trivial.
-                ** specialize (Entropy_addSuccess2 _ 16 _ _ _ _ _ HeqENT32 Heqr); intros XX; simpl in *. 
-                   rewrite XX in HeqMRS; clear XX; inv HeqMRS.
-             -- specialize (Entropy_addError _ 16 _ _ _ HeqENT32); intros XX; simpl in *.
-                rewrite XX in *; clear XX; discriminate.
-  }
-  rewrite H3 in *; clear H3. normalize.   
-  apply andp_right. apply prop_right; repeat split; trivial. 
+  rewrite <- instantiate_reseed in HeqMRS; trivial.
+  rewrite <- HeqMRS.
+  normalize.
+  apply andp_right. apply prop_right; repeat split; trivial.
+  cancel. 
   unfold_data_at 1%nat. cancel.
-Time Qed. (*67.312 secs (53.125u,0.015s) (successful)*)
+  apply deep_interp_empty. 
+Time Qed. (*67.641 secs (57.406u,0.s) (successful)*)
